Lifted the correctness result to the reflexive transitive closure of the compatible closure of the hoisting rewrite relation. Also proved the corollary that states that the hoisting function is correct.

certicoq/theories/L6_PCPS/relations.v
@@ -1,18 +1,22 @@
-Require Import Relations.
+Require Import Relations RelationClasses.
 Require Import cps ctx.
 
 Section Relations.
 
   Variable (R : relation exp).
-
+  (* TODO : abstract over exp ? *)
+  
   Open Scope ctx_scope.
   
+  (** The compatible closure of R *) 
   Inductive compat_closure : relation exp :=
   | Compat :
-      forall c e e',
+      forall e e' c,
         R e e' ->
         compat_closure (c |[ e ]|) (c |[ e' ]|).
-      
+
+  (** The reflexive transitive closure of R, 
+    * parametrized by the numbers of steps *) 
   Inductive refl_trans_closure_n : nat -> relation exp :=
   | Trans :
       forall n e1 e2 e3,
@@ -22,13 +26,32 @@ Section Relations.
   | Refl :
       forall e, refl_trans_closure_n 0 e e.
 
-  Definition invariant (R : relation exp) (I : exp -> Prop)  : Prop :=
+  (** Compatible relation w.r.t to [f] *)
+  Definition Compatible (R' : relation exp) :=
+    forall e1 e2 c,
+      R' e1 e2 -> R' (c |[ e1 ]|) (c |[ e2 ]|).
+   
+  (** Invariant w.r.t. a relation R *)
+  Definition Invariant (R : relation exp) (I : exp -> Prop)  : Prop :=
     forall (e1 e2 : exp),
       I e1 -> R e1 e2 -> I e2.
 
+  (* Better names for these two? *)
+
+  (** If a property if true for [e] then it's true for it's subterms  *)
+  Definition SubtermInvariant (I : exp -> Prop) :=
+    forall c e,  I (c |[ e ]|) ->  I e.
+
+  (** If a property if true for a term and we substitute a subterm [e] with a 
+    * term [e'] such that [R e e'], then it's true for the resulting term  *)
+  Definition SubtermSubstInvariant (R : relation exp) (I : exp -> Prop) :=
+    forall c e e', I (c |[ e ]|) -> R e e' ->  I (c |[ e' ]|).
+
+  (** Lifting of an invariant w.r.t to a relation to the 
+    * reflexive transitive closure of the relation *)
   Lemma invariant_refl_trans_closure (I : exp -> Prop) n :
-    invariant R I ->
-    invariant (refl_trans_closure_n n) I.
+    Invariant R I ->
+    Invariant (refl_trans_closure_n n) I.
   Proof.
     induction n.
     - intros HInv e1 e2 HI Hrw. inv Hrw; eauto.
@@ -36,32 +59,21 @@ Section Relations.
       apply (IHn HInv e3 e2); eauto.
   Qed.
 
-  Definition ctx_compat (I : exp -> Prop) : Prop :=
-    (forall c e e', I (c |[ e ]|) -> I e' ->  I (c |[ e' ]|)) /\
-    (forall c e,  I (c |[ e ]|) ->  I e).
-  
-
-  Lemma invariant_compat_closure (I : exp -> Prop) :
-    invariant R I ->
-    ctx_compat I ->
-    invariant compat_closure I.
+  (** Lifting of an invariant w.r.t to a relation to the 
+    * compatible closure of the relation *)
+  Lemma invariant_compat_closure (R' : relation exp) (I : exp -> Prop) :
+    Invariant R I ->
+    SubtermInvariant I ->
+    SubtermSubstInvariant (fun e e' => R' e e' /\ I e') I ->
+    inclusion _ (fun e e' => R e e' /\ I e) R' -> 
+    Invariant compat_closure I.
   Proof.
-    intros HInv [HS1 HS2] e1 e2 HI Hrw. inv Hrw.
-    eapply HS1; eauto.
+    intros HInv HS1 HS2 HIn e1 e2 HI Hrw. inv Hrw.
+    eapply HS2; eauto. split; eauto.
   Qed.
 
-  Lemma refl_trans_closure_f_compat n e1 e2 f :
-    (forall e1 e2, R e1 e2 -> R (f e1) (f e2)) ->
-    refl_trans_closure_n n e1 e2 ->
-    refl_trans_closure_n n (f e1) (f e2).
-  Proof.
-    revert e1 e2 f. induction n; intros e1 e2 f Hyp H.
-    - inv H. constructor.
-    - inv H. econstructor. apply Hyp. eauto. eauto. 
-  Qed.
-
-  Lemma refl_trans_closure_f_compat_inv n I e1 e2 f :
-    invariant R I ->
+  Lemma refl_trans_closure_f_compat_strong n I e1 e2 f :
+    Invariant R I ->
     (forall e1 e2, I e1 -> R e1 e2 -> R (f e1) (f e2)) ->
     I e1 ->
     refl_trans_closure_n n e1 e2 ->
@@ -74,25 +86,19 @@ Section Relations.
       apply IHn; eauto.
   Qed.
 
-  Lemma refl_trans_closure_R_compat n (R' : relation exp) e1 e2 e1' :
-    (forall e1 e2 e1',
-       R' e1 e1' -> R e1 e2 ->
-       exists e2', R e1' e2' /\ R' e2 e2') ->
-    R' e1 e1' -> 
+
+  Lemma refl_trans_closure_f_compat n e1 e2 f :
+    (forall e1 e2, R e1 e2 -> R (f e1) (f e2)) ->
     refl_trans_closure_n n e1 e2 ->
-    exists e2',
-      R' e2 e2' /\
-      refl_trans_closure_n n e1' e2'.
+    refl_trans_closure_n n (f e1) (f e2).
   Proof.
-    revert e1 e2 e1'. induction n; intros e1 e2 e1' Hyp Hr1 H.
-    - inv H. exists e1'. constructor; eauto. constructor.
-    - inv H. edestruct Hyp as [e3' [Hrw' Hr3]]; eauto.
-      edestruct IHn as [e2' [Hrw Hr2]]; [ | | eauto |]; eauto.
-      eexists. split; eauto. econstructor; eauto.
+    intros. 
+    eapply refl_trans_closure_f_compat_strong with (I := fun _ => True); eauto.
+    intros e1' e2'; eauto. 
   Qed.
 
-  Lemma refl_trans_closure_R_compat_inv n I (R' : relation exp) e1 e2 e1' :
-    invariant R I ->
+  Lemma refl_trans_closure_commut_strong n I (R' : relation exp) e1 e2 e1' :
+    Invariant R I ->
     (forall e1 e2 e1',
        I e1 -> R' e1 e1' -> R e1 e2 ->
        exists e2', R e1' e2' /\ R' e2 e2') ->
@@ -112,6 +118,20 @@ Section Relations.
       eexists. split; eauto. econstructor; eauto.
   Qed.
 
+  Lemma refl_trans_closure_commut n (R' : relation exp) e1 e2 e1' :
+    (forall e1 e2 e1',
+       R' e1 e1' -> R e1 e2 ->
+       exists e2', R e1' e2' /\ R' e2 e2') ->
+    R' e1 e1' -> 
+    refl_trans_closure_n n e1 e2 ->
+    exists e2',
+      R' e2 e2' /\ refl_trans_closure_n n e1' e2'.
+  Proof.
+    intros. 
+    eapply refl_trans_closure_commut_strong with (I := fun _ => True); eauto.
+    intros e1'' e2''; eauto.
+  Qed.
+
 
   Lemma compat_closure_f_compat e1 e2 f :
     (forall e1 e2, R e1 e2 -> R (f e1) (f e2)) ->
@@ -124,16 +144,17 @@ Section Relations.
     destruct (Hyp2 c) as [[c' Heq] | [c' Heq]]; rewrite !Heq; econstructor; eauto.
   Qed.
 
-  Lemma compat_closure_f_compat_inv I e1 e2 f :
-    invariant R I -> ctx_compat I ->
+  Lemma compat_closure_f_compat_inv I (R' : relation exp) e1 e2 f :
+    Invariant R I -> SubtermInvariant I -> SubtermSubstInvariant R' I ->
     (forall e1 e2, I e1 -> R e1 e2 -> R (f e1) (f e2)) ->
     (forall c,  (exists c1, forall e, f (c |[ e ]|) = c1 |[ f e ]|) \/
                 (exists c1, forall e, f (c |[ e ]|) = c1 |[ e ]|)) ->
     I e1 ->
+    inclusion _ R R' ->
     compat_closure e1 e2 ->
     compat_closure (f e1) (f e2).
   Proof.
-    intros Inv [HC1 HC2] Hyp1 Hyp2 HI H. inv H.
+    intros Inv HC1 HC2 Hyp1 Hyp2 HI Hinc H. inv H.
     destruct (Hyp2 c) as [[c' Heq] | [c' Heq]]; rewrite !Heq; econstructor; eauto.
   Qed.
 
@@ -190,5 +211,57 @@ Abort. *)
     intros H. inv H. rewrite !app_ctx_f_fuse.
     constructor; eauto.
   Qed.
+
+  (** If R is included R', and R' is compatible then the 
+      compatible closure of R is in R' *)
+  Lemma relation_inclusion_compat (R' : relation exp) :
+    inclusion _ R R' ->
+    Compatible R' ->
+    inclusion _ compat_closure R'.
+  Proof.
+    intros Hyp1 Hyp2 e1 e2 Hcomp. inv Hcomp. eauto.
+  Qed.
   
+  (** If R is included R', and R' is reflexive and transitive then the 
+      reflexive transitive closure of R is in R' *)
+  Lemma relation_inclusion_refl_trans (R' : relation exp) n :
+    (forall e1 e2, R e1 e2 -> R' e1 e2) ->
+    Reflexive R' ->
+    Transitive R' ->
+    inclusion _ (refl_trans_closure_n n) R'.  
+  Proof.
+    intros Hyp1 Hrefl Htrans e1 e2 Hstar. induction Hstar; eauto.
+  Qed.
+
+  (** If R is included R', and R' is compatible then the 
+      compatible closure of R is in R' *)
+  Lemma relation_inclusion_compat_strong (Pre : exp -> Prop)
+        (R' : relation exp) e1 e2 :
+    (forall e1 e2, Pre e1 -> R e1 e2 -> R' e1 e2) ->
+    Pre e1 ->
+    SubtermInvariant Pre ->
+    Compatible R' ->
+    compat_closure e1 e2 ->
+    R' e1 e2.
+  Proof.
+    intros H1 H2 H3 H4 Hcomp. inv Hcomp. eauto.
+  Qed.
+  
+  (** If R is included R', and R' is reflexive and transitive then the 
+      reflexive transitive closure of R is in R' *)  
+  Lemma relation_inclusion_refl_trans_strong (Pre : exp -> Prop)
+        (R' : relation exp) e1 e2 n :
+    (forall e1 e2, Pre e1 -> R e1 e2 -> R' e1 e2) ->
+    Pre e1 ->
+    Invariant R Pre ->
+    (forall e, Pre e -> R' e e) ->
+    (forall e1 e2 e3, Pre e1 -> Pre e2 -> R' e1 e2 -> R' e2 e3 -> R' e1 e3) ->
+    refl_trans_closure_n n e1 e2 ->
+    R' e1 e2.
+  Proof.
+    intros H1 H2 H3 Hrefl Htrans Hstar. induction Hstar; eauto.
+    eapply Htrans. eauto. eapply H3. eassumption. eassumption.
+    now eauto. eapply IHHstar. eauto.
+  Qed.
+
 End Relations.
